# Product Rule

If `f(x) = a(x)*b(x)`, then `f'(x) = a'(x)*b(x) + a(x)*b'(x)` (at all points where `a'(x)` and `b'(x)` are defined). 

If `f(x) = a(x)*b(x)*c(x)`, then `f'(x) = a'(x)*b(x)*c(x) + a(x)*b'(x)*c(x) + a(x)*b(x)*c'(x)` (at all points where `a'(x)`, `b'(x)`, and `c'(x)` are defined). 

If `f(x) = a(x)*b(x)*c(x)*d(x)`, then `f'(x) = a'(x)*b(x)*c(x)*d(x) + a(x)*b'(x)*c(x)*d(x) + a(x)*b(x)*c'(x)*d(x) + a(x)*b(x)*c(x)*d'(x)` (at all points where `a'(x)`, `b'(x)`, `c'(x)`, and `d'(x)` are defined). 

