# Calculating derivatives

If `g(x) = k*f(x)` for all `x`, then `g'(x) = k*f'x)`

***

If `f(x) = -3/x`, then what is `f'(x)`?

`-3 / x^1`

`-3 * x^(-1)`

`-3 * (-1) * x^(-2)`

**`f'(x) = 3 / (x^2)`**

***

The derivative of a sum is equal to the sum of the derivatives. 

***

If `f(x) = x^2 - (1/x)`, then what is `f'(x)`?

Using the above sum-of-derivatives rule, we can break this down into sub-problems:

`f'(x) = f'(x^2) - f'(1/x)`

`= 2x - f'(1 * x(^-1))`

`= 2x - (-1 * x^-2)`

`= 2x + 1/(x^2)`

***

## The Power Rule

`f(x) = x^n` means that `f'(x) = n*x^(n-1)`. 

`n` may be any fixed number, and the base `x` must be the input variable for the function. 

***

 ![image](https://github.com/user-attachments/assets/d21adcf7-244c-457b-9351-217306f7700d)

